theories/tests/readonly.v
@@ -51,7 +51,7 @@ Section proof.
 End proof.
 
 Lemma usetwo_safe C t2 σ2 :
-  adv_ctx C →
+  AdvCtx C →
   rtc step ([ctx_fill C usetwo], good_state ∅) (t2, σ2) →
   is_good σ2.
 Proof.
